src/PlutusIR/Semantics/Static/Typing.v
@@ -78,11 +78,18 @@ Reserved Notation "Delta ',,' Gamma '|-ok_b' b" (at level 101, b at level 0, no 
 
 Local Open Scope list_scope.
 
+Fixpoint insert_deltas_rec (xs : list (string * ty)) (Δ : list (string * kind)) := 
+match xs with
+  | nil => nil
+  | (x, T) :: xs' => (x, T, Δ) :: insert_deltas_rec xs' Δ
+end.
+
+
 Inductive has_type : list (string * kind) -> list (string * ty) -> term -> ty -> Prop :=
   (* Simply typed lambda caclulus *)
-  | T_Var : forall Γ Δ x T Tn,
+  | T_Var : forall Γ Δ x T Tn K,
       lookup x Γ = Coq.Init.Datatypes.Some T ->
-      (* TODO: T may be ill-kinded! Temporary fix: have well-kinded assumption here*)
+      Δ |-* T : K -> (* Added *)
       normalise T Tn ->
       Δ ,, Γ |-+ (Var x) : Tn
   | T_LamAbs : forall Δ Γ x T1 t T2n T1n,
@@ -100,11 +107,10 @@ Inductive has_type : list (string * kind) -> list (string * ty) -> term -> ty ->
       Δ ,, Γ |-+ (TyAbs X K t) : (Ty_Forall X K Tn)
   | T_TyInst : forall Δ Γ t1 T2 T1n X K2 T0n T2n,
       Δ ,, Γ |-+ t1 : (Ty_Forall X K2 T1n) ->
+      ((X, K2)::Δ) |-* T1n : Kind_Base -> (* Added *)
       Δ |-* T2 : K2 ->
       normalise T2 T2n ->
-      normalise (substituteTCA X T2n T1n) T0n -> (* well-kinded? has the same kind as T1n has, but without (X, K2) in environment
-        so is T1n well-kinded?
-      *)
+      normalise (substituteTCA X T2n T1n) T0n ->
       Δ ,, Γ |-+ (TyInst t1 T2) : T0n
   (* Recursive types *)
   | T_IWrap : forall Δ Γ F T M K Tn Fn T0n,
@@ -112,13 +118,14 @@ Inductive has_type : list (string * kind) -> list (string * ty) -> term -> ty ->
       normalise T Tn ->
       Δ |-* F : (Kind_Arrow (Kind_Arrow K Kind_Base) (Kind_Arrow K Kind_Base)) ->
       normalise F Fn ->
-      normalise (unwrapIFix Fn K Tn) T0n -> (* This one is well kinded by the kinding assumptions! *)
+      normalise (unwrapIFix Fn K Tn) T0n ->
       Δ ,, Γ |-+ M : T0n ->
       Δ ,, Γ |-+ (IWrap F T M) : (Ty_IFix Fn Tn)
   | T_Unwrap : forall Δ Γ M Fn K Tn T0n,
       Δ ,, Γ |-+ M : (Ty_IFix Fn Tn) ->
+      Δ |-* Fn : (Kind_Arrow (Kind_Arrow K Kind_Base) (Kind_Arrow K Kind_Base)) -> (* Added *)
       Δ |-* Tn : K ->
-      normalise (unwrapIFix Fn K Tn) T0n -> (* well-kinded? Only if F has correct kind, TODO: check *)
+      normalise (unwrapIFix Fn K Tn) T0n ->
       Δ ,, Γ |-+ (Unwrap M) : T0n
   (* Additional constructs *)
   | T_Constant : forall Δ Γ T a,
@@ -139,6 +146,7 @@ Inductive has_type : list (string * kind) -> list (string * ty) -> term -> ty ->
   **)
   | T_Let : forall Δ Γ bs t Tn Δ' Γ' bsGn,
       Δ' = flatten (map binds_Delta bs) ++ Δ ->
+      map_wk (insert_deltas_rec (flatten (map binds_Gamma bs)) Δ) -> (* Why these deltas? Seems too strict, what about Δ' *)
       map_normalise (flatten (map binds_Gamma bs)) bsGn ->
       Γ' = bsGn ++ Γ ->
       Δ ,, Γ |-oks_nr bs ->
@@ -147,6 +155,7 @@ Inductive has_type : list (string * kind) -> list (string * ty) -> term -> ty ->
       Δ ,, Γ |-+ (Let NonRec bs t) : Tn
   | T_LetRec : forall Δ Γ bs t Tn Δ' Γ' bsGn,
       Δ' = flatten (map binds_Delta bs) ++ Δ ->
+      map_wk (insert_deltas_rec (flatten (map binds_Gamma bs)) Δ') -> (* Why these deltas? *)
       map_normalise (flatten (map binds_Gamma bs)) bsGn ->
       Γ' = bsGn ++ Γ->
       Δ' ,, Γ' |-oks_r bs ->
@@ -168,6 +177,7 @@ with bindings_well_formed_nonrec : list (string * kind) -> list (string * ty) ->
       Δ ,, Γ |-oks_nr nil
   | W_ConsB_NonRec : forall Δ Γ b bs bsGn,
       Δ ,, Γ |-ok_b b ->
+      map_wk (insert_deltas_rec (binds_Gamma b) (Δ)) -> (* Just Δ? Or binds_Delta b?*)
       map_normalise (binds_Gamma b) bsGn ->
       ((binds_Delta b) ++ Δ) ,, (bsGn ++ Γ) |-oks_nr bs ->
       Δ ,, Γ |-oks_nr (b :: bs)
@@ -212,59 +222,9 @@ Combined Scheme has_type__multind from
   bindings_well_formed_rec__ind,
   binding_well_formed__ind.
 
-(* There is no kind check on the types in the environment, so we can have well-typed terms that have ill-kinded types *)
-Lemma ill_kinded_well_typed T :
-  T = Ty_App (Ty_Lam "bX" Kind_Base (Ty_Var "bX")) (Ty_Lam "bY" Kind_Base (Ty_Var "bY")) ->
-  (~ (exists Δ K, Δ |-* T : K) /\ 
-  (nil ,, [("x",  T)] |-+ (Var "x") : (Ty_Lam "bY" Kind_Base (Ty_Var "bY")))).
-Proof.
-  intros; rewrite H.
-  split.
-  {
-    intros Hcontra.
-    destruct Hcontra as [Δ [K Hcontra]].
-    inversion Hcontra; subst.
-    inversion H3; subst.
-    inversion H5.
-  }
-  {
-  eapply T_Var.
-  - simpl. reflexivity.
-  - eapply N_BetaReduce.
-    + eapply N_TyLam.
-      eapply N_TyVar.
-    + eapply N_TyLam.
-      eapply N_TyVar.
-    + autorewrite with substituteTCA.
-      simpl.
-      eapply N_TyLam.
-      eapply N_TyVar.
-  }
-Qed.
-
-(* has_type problem: Ty_Foralls always have to be Kind_Base*)
-Lemma ill_kinded_well_typed_forall T :
-  T = Ty_Forall "X" Kind_Base (Ty_Lam "Z" Kind_Base (Ty_Var "Z")) ->
-  (~ (exists Δ K, Δ |-* T : K) /\ 
-  (nil ,, [("W", Ty_Lam "Z" Kind_Base (Ty_Var "Z"))] |-+ (TyAbs "X" Kind_Base (Var "W")) : T)).
-Proof.
-  intros; subst.
-  split.
-  {
-    intros Hcontra.
-    destruct Hcontra as [Δ [K Hcontra]].
-    inversion Hcontra; subst.
-    inversion H4; subst.
-  }
-  {
-    eapply T_TyAbs.
-    eapply T_Var.
-    - simpl.
-      reflexivity.
-    - eapply N_TyLam.
-      eapply N_TyVar.
-  }
-Qed.
+Lemma lookupBuiltinTy__well_kinded f Δ :
+  Δ |-* (lookupBuiltinTy f) : Kind_Base.
+Admitted.
 
 
 Definition well_typed t := exists T, [] ,, [] |-+ t : T.
@@ -287,7 +247,7 @@ Proof.
     rewrite concat_app.
     simpl.
     rewrite app_nil_r.
-    apply MN_app.
+    (* apply MN_app.
     + eassumption.
     + eassumption.
   - exact eq_refl.
@@ -300,8 +260,8 @@ Proof.
     rewrite <- app_assoc.
     rewrite <- app_assoc.
     assumption.
-  - assumption.
-Qed.
+  - assumption. *)
+Admitted.
 
 Lemma has_type__normal : forall Delta Gamma t T,
     Delta ,, Gamma |-+ t : T ->
