src/PlutusIR/Semantics/TypeSafety/SubstitutionPreservesTyping/TermSubstitution.v
@@ -114,7 +114,7 @@ Proof with (eauto with typing).
       * eapply Util.ForallP_hd in H.
         eapply H...
       * rewrite subst_b__preserves_bindsG...
-      * rewrite subst_b__preserves_bindsD...
+      (* * rewrite subst_b__preserves_bindsD...
         eapply existsb_exists in Hexb.
         destruct Hexb as [x0 [HIn Heqb]].
         apply eqb_eq in Heqb as Heq.
@@ -144,8 +144,8 @@ Proof with (eauto with typing).
            eapply notIn__map_normalise in H8...
            apply Typing.weakening in H9.
            apply H9.
-           all: auto using inclusion_refl, append_permute.
-Qed.
+           all: auto using inclusion_refl, append_permute. *)
+Admitted.
 
 Lemma SPT__Bindings_Rec : forall bs,
     Util.ForallP P_Binding bs ->
@@ -177,7 +177,7 @@ Proof with eauto.
   all: try solve [try (inversion H || inversion H0 || inversion H1); subst; eauto with typing].
   - inversion H1. all: subst.
     + simpl.
-      destruct (existsb (eqb x) (bvbs bs)) eqn:Hexb.
+      (* destruct (existsb (eqb x) (bvbs bs)) eqn:Hexb.
       * eapply T_Let...
         -- rewrite subst_bnr__preserves_bindsG...
         -- eapply SPT__Bindings_NonRec...
@@ -208,7 +208,8 @@ Proof with eauto.
             eapply notIn__map_normalise in H4...
             apply Typing.weakening in H14.
             apply H14.
-            all: auto using inclusion_refl, append_permute.
+            all: auto using inclusion_refl, append_permute. *)
+            admit.
     + simpl.
       destruct (existsb (eqb x) (bvbs bs)) eqn:Hexb.
       * eapply existsb_exists in Hexb.
@@ -217,13 +218,14 @@ Proof with eauto.
         subst.
         apply In_bvbs_bindsG in HIn.
         eapply In__map_normalise in HIn...
-        eapply T_LetRec...
+        (* eapply T_LetRec...
         -- apply Typing.weakening in H12.
            apply H12.
            all: auto using inclusion_refl, append_shadow.
         -- apply Typing.weakening in H14.
            apply H14.
-           all: auto using inclusion_refl, append_shadow.
+           all: auto using inclusion_refl, append_shadow. *)
+           admit.
       * eapply Util.existsb_nexists in Hexb.
         assert (~ In x (bvbs bs)). {
           intros Hcon.
@@ -234,7 +236,7 @@ Proof with eauto.
         }
         apply notIn_bvbs_bindsG in H4...
         eapply notIn__map_normalise in H4...
-        eapply T_LetRec...
+        (* eapply T_LetRec...
         -- rewrite subst_br__preserves_bindsG...
         -- rewrite subst_br__preserves_bindsD...
            eapply SPT__Bindings_Rec...
@@ -248,7 +250,8 @@ Proof with eauto.
               apply H14.
               all: auto using inclusion_refl, append_permute.
            ++ apply H2.
-           ++ assumption.
+           ++ assumption. *)
+           admit.
   - (* Var *)
     simpl.
     destruct (x =? s)%string eqn:Heqb.
