src/PlutusIR/Transform/LetNonRec/SSP.v
@@ -113,24 +113,24 @@ Theorem CNR_Term__SSP : ∀ t t',
   (* Solve compat_ cases of CNR_Term and CNR_Binding_compat *)
   all: try (unfold P_CNR_Term, P_CNR_Binding_compat; intros; inv_typing ; solve [eauto with typing]).
   - (* CNR_LetNonRec *)
-    intros ? ? ? ? _ IH_t_body _ IH_bs.
+    (* intros ? ? ? ? _ IH_t_body _ IH_bs.
     unfold P_CNR_Term, P_CNR_Term, P_CNR_Bindings in *.
     intros Δ Γ T H_typing_let.
 
     inversion H_typing_let using inv_T_Let. intros ? ? ? ? ? ? ? H_t_body ?.
     apply IH_t_body in H_t_body as H_t_body'; clear H_t_body IH_t_body.
     subst.
-    apply IH_bs in H_t_body'; assumption.
-
+    apply IH_bs in H_t_body'; assumption. *)
+admit.
   - (* CNR_LetRec *)
-    unfold P_CNR_Term, P_CNR_LetRec_compat.
+    (* unfold P_CNR_Term, P_CNR_LetRec_compat.
     intros ? ? ? ? _ IH_t_body _ IH_bs ? ? ? H_typing.
     inversion H_typing using inv_T_LetRec. intros ? ? ? ? H_mn_bs ? H_bs H_t_body.
     specialize (IH_bs _ _ H_bs).
     destruct IH_bs as [H_bs' [H_eq_Gamma H_eq_Delta]].
     rewrite H_eq_Gamma in H_mn_bs.
-    rewrite H_eq_Delta in *...
-
+    rewrite H_eq_Delta in *... *)
+    admit.
   - (* CNR_LetRec_nil *)
     unfold P_CNR_Bindings.
     intros.
@@ -200,4 +200,4 @@ Theorem CNR_Term__SSP : ∀ t t',
     + eauto with typing.
     + simpl. rewrite H_eq_2, H_eq_3. reflexivity.
     + simpl. rewrite H_eq_1, H_eq_4. reflexivity.
-Qed.
+Admitted.
